ModularEngine/src/LogicEngine.FStar/prims.fst
@@ -175,14 +175,19 @@ extern Runtime val string_of_any_for_coq_afn : 'a -> string
 extern Runtime val writeToFile : string -> 'a -> string
 extern Runtime val writeCertToFile : string -> 'a -> string
 extern Runtime val print_int : int -> bool
-extern Runtime val strcat : string -> string -> string
+
+logic function Strcat : string -> string -> string
+logic function ReprInt: int -> string
+extern Runtime val strcat : s1:string -> s2:string -> r:string{(Strcat s1 s2) = r}
 extern Runtime val strStartsWith: string -> string -> bool
 extern Runtime val strSubstring: string -> int -> int -> string
 extern Runtime val strSubstringNoLength: string -> int -> string
 extern Runtime val strIndexOf: string -> string -> int
-extern Runtime val strLength: string -> int
-extern Runtime val intToString: int -> string
-extern Runtime val stringToInt: string -> int
+extern Runtime val strLength: s:string -> int
+extern Runtime val intToString: n:int -> s:string{s=(ReprInt n)}
+extern Runtime val stringToInt: s:string -> n:int{s=(ReprInt n)}
+extern Runtime val strRmPfx: s:string -> pfx:string -> r:string{s=(Strcat pfx r)}
+extern Runtime val strSplitByDelimiter: s:string -> d:string -> (r1:string*r2:string{s=(Strcat r1 r2)})
 
 extern Runtime val boxToObject: 'a -> object
 extern Runtime val addBindings: object -> string -> bool
